PropositionalLogic/Sound/Sound_Kripke.v
@@ -15,7 +15,21 @@ Import PropositionalLanguageNotation.
 Import KripkeModelFamilyNotation.
 Import KripkeModelNotation_Intuitionistic.
 
-Lemma sound_modus_ponens {L: Language} {nL: NormalLanguage L} {pL: PropositionalLanguage L} {MD: Model} {kMD: KripkeModel MD} {M: Kmodel} {R: Relation (Kworlds M)} {po_R: PreOrder Krelation} {SM: Semantics L MD} {kiSM: KripkeIntuitionisticSemantics L MD M SM}:
+Section Sound_Kripke.
+
+Context {L: Language}
+        {nL: NormalLanguage L}
+        {pL: PropositionalLanguage L}
+        {MD: Model}
+        {kMD: KripkeModel MD}
+        {M: Kmodel}
+        {R: Relation (Kworlds M)}
+        {po_R: PreOrder Krelation}
+        {SM: Semantics L MD}
+        {kiSM: KripkeIntuitionisticSemantics L MD M SM}
+        {kpSM: KripkePropositionalSemantics L MD M SM}.
+
+Lemma sound_modus_ponens:
   forall x y: expr,
     forall m,
       KRIPKE: M, m |= (x --> y) -> KRIPKE: M, m |= x -> KRIPKE: M, m |= y.
@@ -27,7 +41,7 @@ Proof.
   reflexivity.
 Qed.
 
-Lemma sound_axiom1 {L: Language} {nL: NormalLanguage L} {pL: PropositionalLanguage L} {MD: Model} {kMD: KripkeModel MD} {M: Kmodel} {R: Relation (Kworlds M)} {po_R: PreOrder Krelation} {SM: Semantics L MD} {kiSM: KripkeIntuitionisticSemantics L MD M SM}:
+Lemma sound_axiom1:
   forall x y: expr,
     forall m,
       KRIPKE: M, m |= x --> y --> x.
@@ -38,7 +52,7 @@ Proof.
   eapply sat_mono; eauto.
 Qed.
 
-Lemma sound_axiom2 {L: Language} {nL: NormalLanguage L} {pL: PropositionalLanguage L} {MD: Model} {kMD: KripkeModel MD} {M: Kmodel} {R: Relation (Kworlds M)} {po_R: PreOrder Krelation} {SM: Semantics L MD} {kiSM: KripkeIntuitionisticSemantics L MD M SM}:
+Lemma sound_axiom2:
   forall x y z: expr,
     forall m,
       KRIPKE: M, m |= (x --> y --> z) --> (x --> y) --> (x --> z).
@@ -59,7 +73,7 @@ Proof.
   auto.
 Qed.
 
-Lemma sound_andp_intros {L: Language} {nL: NormalLanguage L} {pL: PropositionalLanguage L} {MD: Model} {kMD: KripkeModel MD} {M: Kmodel} {R: Relation (Kworlds M)} {po_R: PreOrder Krelation} {SM: Semantics L MD} {kiSM: KripkeIntuitionisticSemantics L MD M SM}:
+Lemma sound_andp_intros:
   forall x y: expr,
     forall m,
       KRIPKE: M, m |= x --> y --> x && y.
@@ -73,7 +87,7 @@ Proof.
   + auto.
 Qed.
 
-Lemma sound_andp_elim1 {L: Language} {nL: NormalLanguage L} {pL: PropositionalLanguage L} {MD: Model} {kMD: KripkeModel MD} {M: Kmodel} {R: Relation (Kworlds M)} {po_R: PreOrder Krelation} {SM: Semantics L MD} {kiSM: KripkeIntuitionisticSemantics L MD M SM}:
+Lemma sound_andp_elim1:
   forall x y: expr,
     forall m,
       KRIPKE: M, m |= x && y --> x.
@@ -84,7 +98,7 @@ Proof.
   tauto.
 Qed.
 
-Lemma sound_andp_elim2 {L: Language} {nL: NormalLanguage L} {pL: PropositionalLanguage L} {MD: Model} {kMD: KripkeModel MD} {M: Kmodel} {R: Relation (Kworlds M)} {po_R: PreOrder Krelation} {SM: Semantics L MD} {kiSM: KripkeIntuitionisticSemantics L MD M SM}:
+Lemma sound_andp_elim2:
   forall x y: expr,
     forall m,
       KRIPKE: M, m |= x && y --> y.
@@ -95,7 +109,7 @@ Proof.
   tauto.
 Qed.
 
-Lemma sound_orp_intros1 {L: Language} {nL: NormalLanguage L} {pL: PropositionalLanguage L} {MD: Model} {kMD: KripkeModel MD} {M: Kmodel} {R: Relation (Kworlds M)} {po_R: PreOrder Krelation} {SM: Semantics L MD} {kiSM: KripkeIntuitionisticSemantics L MD M SM}:
+Lemma sound_orp_intros1:
   forall x y: expr,
     forall m,
       KRIPKE: M, m |= x --> x || y.
@@ -106,7 +120,7 @@ Proof.
   tauto.
 Qed.
 
-Lemma sound_orp_intros2 {L: Language} {nL: NormalLanguage L} {pL: PropositionalLanguage L} {MD: Model} {kMD: KripkeModel MD} {M: Kmodel} {R: Relation (Kworlds M)} {po_R: PreOrder Krelation} {SM: Semantics L MD} {kiSM: KripkeIntuitionisticSemantics L MD M SM}:
+Lemma sound_orp_intros2:
   forall x y: expr,
     forall m,
       KRIPKE: M, m |= y --> x || y.
@@ -117,7 +131,7 @@ Proof.
   tauto.
 Qed.
 
-Lemma sound_orp_elim {L: Language} {nL: NormalLanguage L} {pL: PropositionalLanguage L} {MD: Model} {kMD: KripkeModel MD} {M: Kmodel} {R: Relation (Kworlds M)} {po_R: PreOrder Krelation} {SM: Semantics L MD} {kiSM: KripkeIntuitionisticSemantics L MD M SM}:
+Lemma sound_orp_elim:
   forall x y z: expr,
     forall m,
       KRIPKE: M, m |= (x --> z) --> (y --> z) --> (x || y --> z).
@@ -135,7 +149,7 @@ Proof.
     apply H2; auto.
 Qed.
 
-Lemma sound_falsep_elim {L: Language} {nL: NormalLanguage L} {pL: PropositionalLanguage L} {MD: Model} {kMD: KripkeModel MD} {M: Kmodel} {R: Relation (Kworlds M)} {po_R: PreOrder Krelation} {SM: Semantics L MD} {kiSM: KripkeIntuitionisticSemantics L MD M SM}:
+Lemma sound_falsep_elim:
   forall x: expr,
     forall m,
       KRIPKE: M, m |= FF --> x.
@@ -146,7 +160,7 @@ Proof.
   tauto.
 Qed.
 
-Lemma sound_excluded_middle_ident {L: Language} {nL: NormalLanguage L} {pL: PropositionalLanguage L} {MD: Model} {kMD: KripkeModel MD} {M: Kmodel} {R: Relation (Kworlds M)} {po_R: PreOrder Krelation} {ikiM: IdentityKripkeIntuitionisticModel (Kworlds M)} {SM: Semantics L MD} {kiSM: KripkeIntuitionisticSemantics L MD M SM}:
+Lemma sound_excluded_middle_ident {ikiM: IdentityKripkeIntuitionisticModel (Kworlds M)}:
   forall x: expr,
     forall m, KRIPKE: M, m |= x || ~~ x.
 Proof.
@@ -159,7 +173,7 @@ Proof.
   tauto.
 Qed.
 
-Lemma sound_impp_choice_no_branch {L: Language} {nL: NormalLanguage L} {pL: PropositionalLanguage L} {MD: Model} {kMD: KripkeModel MD} {M: Kmodel} {R: Relation (Kworlds M)} {po_R: PreOrder Krelation} {nkiM: NoBranchKripkeIntuitionisticModel (Kworlds M)} {SM: Semantics L MD} {kiSM: KripkeIntuitionisticSemantics L MD M SM}:
+Lemma sound_impp_choice_no_branch {nkiM: NoBranchKripkeIntuitionisticModel (Kworlds M)}:
   forall x y: expr,
     forall m, KRIPKE: M, m |= (x --> y) || (y --> x).
 Proof.
@@ -183,7 +197,7 @@ Proof.
     tauto.
 Qed.
 
-Lemma sound_weak_excluded_middle_branch_join {L: Language} {nL: NormalLanguage L} {pL: PropositionalLanguage L} {MD: Model} {kMD: KripkeModel MD} {M: Kmodel} {R: Relation (Kworlds M)} {po_R: PreOrder Krelation} {bkiM: BranchJoinKripkeIntuitionisticModel (Kworlds M)} {SM: Semantics L MD} {kiSM: KripkeIntuitionisticSemantics L MD M SM}:
+Lemma sound_weak_excluded_middle_branch_join {bkiM: BranchJoinKripkeIntuitionisticModel (Kworlds M)}:
   forall x: expr,
     forall m, KRIPKE: M, m |= ~~ x || ~~ ~~ x.
 Proof.
@@ -208,3 +222,5 @@ Proof.
   apply (H2 n) in H1; [| reflexivity].
   apply sat_falsep in H1; auto.
 Qed.
+
+End Sound_Kripke.
