SeparationLogic/Sound/Sound_DownUp_Fail.v
@@ -18,7 +18,7 @@ Import SeparationLogicNotation.
 Import KripkeModelFamilyNotation.
 Import KripkeModelNotation_Intuitionistic.
 
-Lemma sound_sepcon_comm {L: Language} {nL: NormalLanguage L} {pL: PropositionalLanguage L} {sL: SeparationLanguage L} {MD: Model} {kMD: KripkeModel MD} (M: Kmodel) {R: Relation (Kworlds M)} {po_R: PreOrder Krelation} {J: Join (Kworlds M)} {SA: SeparationAlgebra (Kworlds M)} {SM: Semantics L MD} {kiSM: KripkeIntuitionisticSemantics L MD M SM} {dusSM: DownUpSemantics_Fail.SeparatingSemantics L MD M SM}:
+Lemma sound_sepcon_comm {L: Language} {nL: NormalLanguage L} {pL: PropositionalLanguage L} {sL: SeparationLanguage L} {MD: Model} {kMD: KripkeModel MD} (M: Kmodel) {R: Relation (Kworlds M)} {po_R: PreOrder Krelation} {J: Join (Kworlds M)} {SA: SeparationAlgebra (Kworlds M)} {SM: Semantics L MD} {kiSM: KripkeIntuitionisticSemantics L MD M SM} {kpSM: KripkePropositionalSemantics L MD M SM} {dusSM: DownUpSemantics_Fail.SeparatingSemantics L MD M SM}:
   forall x y: expr,
     forall m,
       KRIPKE: M, m |= x * y --> y * x.
@@ -32,7 +32,7 @@ Proof.
   apply join_comm; auto.
 Qed.
 
-Lemma sound_sepcon_assoc {L: Language} {nL: NormalLanguage L} {pL: PropositionalLanguage L} {sL: SeparationLanguage L} {MD: Model} {kMD: KripkeModel MD} (M: Kmodel) {R: Relation (Kworlds M)} {po_R: PreOrder Krelation} {J: Join (Kworlds M)} {SA: SeparationAlgebra (Kworlds M)} {SM: Semantics L MD} {kiSM: KripkeIntuitionisticSemantics L MD M SM} {dusSM: DownUpSemantics_Fail.SeparatingSemantics L MD M SM}:
+Lemma sound_sepcon_assoc {L: Language} {nL: NormalLanguage L} {pL: PropositionalLanguage L} {sL: SeparationLanguage L} {MD: Model} {kMD: KripkeModel MD} (M: Kmodel) {R: Relation (Kworlds M)} {po_R: PreOrder Krelation} {J: Join (Kworlds M)} {SA: SeparationAlgebra (Kworlds M)} {SM: Semantics L MD} {kiSM: KripkeIntuitionisticSemantics L MD M SM} {kpSM: KripkePropositionalSemantics L MD M SM} {dusSM: DownUpSemantics_Fail.SeparatingSemantics L MD M SM}:
   forall x y z: expr,
     forall m,
       KRIPKE: M, m |= x * (y * z) <--> (x * y) * z.
