SeparationLogic/Sound/Sound_Flat.v
@@ -18,7 +18,27 @@ Import SeparationLogicNotation.
 Import KripkeModelFamilyNotation.
 Import KripkeModelNotation_Intuitionistic.
 
-Lemma sound_sepcon_comm {L: Language} {nL: NormalLanguage L} {pL: PropositionalLanguage L} {sL: SeparationLanguage L} {MD: Model} {kMD: KripkeModel MD} (M: Kmodel) {R: Relation (Kworlds M)} {po_R: PreOrder Krelation} {J: Join (Kworlds M)} {SA: SeparationAlgebra (Kworlds M)} {SM: Semantics L MD} {kiSM: KripkeIntuitionisticSemantics L MD M SM} {fsSM: SeparatingSemantics L MD M SM}:
+Section Sound_Flat.
+
+Context {L: Language}
+        {nL: NormalLanguage L}
+        {pL: PropositionalLanguage L}
+        {sL: SeparationLanguage L}
+        {MD: Model}
+        {kMD: KripkeModel MD}
+        (M: Kmodel)
+        {R: Relation (Kworlds M)}
+        {po_R: PreOrder Krelation}
+        {J: Join (Kworlds M)}
+        {SA: SeparationAlgebra (Kworlds M)}
+        {uSA: UpwardsClosedSeparationAlgebra (Kworlds M)}
+        {dSA: DownwardsClosedSeparationAlgebra (Kworlds M)}
+        {SM: Semantics L MD}
+        {kiSM: KripkeIntuitionisticSemantics L MD M SM}
+        {kpSM: KripkePropositionalSemantics L MD M SM}
+        {fsSM: FlatSemantics.SeparatingSemantics L MD M SM}.
+
+Lemma sound_sepcon_comm:
   forall x y: expr,
     forall m,
       KRIPKE: M, m |= x * y --> y * x.
@@ -32,7 +52,7 @@ Proof.
   apply join_comm; auto.
 Qed.
 
-Lemma sound_sepcon_assoc {L: Language} {nL: NormalLanguage L} {pL: PropositionalLanguage L} {sL: SeparationLanguage L} {MD: Model} {kMD: KripkeModel MD} (M: Kmodel) {R: Relation (Kworlds M)} {po_R: PreOrder Krelation} {J: Join (Kworlds M)} {SA: SeparationAlgebra (Kworlds M)} {SM: Semantics L MD} {kiSM: KripkeIntuitionisticSemantics L MD M SM} {fsSM: SeparatingSemantics L MD M SM}:
+Lemma sound_sepcon_assoc:
   forall x y z: expr,
     forall m,
       KRIPKE: M, m |= x * (y * z) <--> (x * y) * z.
@@ -71,7 +91,7 @@ Proof.
     split; [| split]; auto.
 Qed.
 
-Lemma sound_wand_sepcon_adjoint {L: Language} {nL: NormalLanguage L} {pL: PropositionalLanguage L} {sL: SeparationLanguage L} {MD: Model} {kMD: KripkeModel MD} (M: Kmodel) {R: Relation (Kworlds M)}  {po_R: PreOrder Krelation} {J: Join (Kworlds M)} {SA: SeparationAlgebra (Kworlds M)} {SM: Semantics L MD} {kiSM: KripkeIntuitionisticSemantics L MD M SM} {fsSM: SeparatingSemantics L MD M SM}:
+Lemma sound_wand_sepcon_adjoint:
   forall x y z: expr,
     (forall m, KRIPKE: M, m |= x * y --> z) <-> (forall m, KRIPKE: M, m |= x --> (y -* z)).
 Proof.
@@ -107,7 +127,7 @@ Proof.
     apply (ASSU m2 n m1); auto.
 Qed.
 
-Lemma sound_sepcon_mono {L: Language} {nL: NormalLanguage L} {pL: PropositionalLanguage L} {sL: SeparationLanguage L} {MD: Model} {kMD: KripkeModel MD} (M: Kmodel) {R: Relation (Kworlds M)}  {po_R: PreOrder Krelation} {J: Join (Kworlds M)} {SA: SeparationAlgebra (Kworlds M)} {SM: Semantics L MD} {kiSM: KripkeIntuitionisticSemantics L MD M SM} {fsSM: SeparatingSemantics L MD M SM}:
+Lemma sound_sepcon_mono:
   forall x1 x2 y1 y2: expr,
    (forall m, KRIPKE: M, m |= x1 --> x2) ->
    (forall m, KRIPKE: M, m |= y1 --> y2) ->
@@ -134,7 +154,23 @@ Proof.
   exists m1, m2; auto.
 Qed.
 
-Lemma sound_sepcon_emp {L: Language} {nL: NormalLanguage L} {pL: PropositionalLanguage L} {sL: SeparationLanguage L} {s'L: SeparationEmpLanguage L} {MD: Model} {kMD: KripkeModel MD} (M: Kmodel) {R: Relation (Kworlds M)}  {po_R: PreOrder Krelation} {J: Join (Kworlds M)} {SA: SeparationAlgebra (Kworlds M)} {USA: UnitalSeparationAlgebra (Kworlds M)} {SM: Semantics L MD} {kiSM: KripkeIntuitionisticSemantics L MD M SM} {fsSM: SeparatingSemantics L MD M SM} {feSM: EmpSemantics L MD M SM}:
+Lemma sound_sepcon_elim1 {incrSA: IncreasingSeparationAlgebra (Kworlds M)}:
+  forall x y: expr,
+    forall m, KRIPKE: M, m |= x * y --> x.
+Proof.
+  intros.
+  rewrite sat_impp; intros.
+  rewrite sat_sepcon in H0.
+  destruct H0 as [m1 [m2 [? [? ?]]]].
+  apply join_comm in H0.
+  apply all_increasing in H0.
+  eapply sat_mono; eauto.
+Qed.
+
+Context {s'L: SeparationEmpLanguage L}
+        {feSM: EmpSemantics L MD M SM}.
+
+Lemma sound_sepcon_emp {USA: UnitalSeparationAlgebra (Kworlds M)}:
   forall x: expr,
     forall m, KRIPKE: M, m |= x * emp <--> x.
 Proof.
@@ -161,7 +197,7 @@ Proof.
     - rewrite sat_emp; auto.
 Qed.
 
-Lemma sound_emp_sepcon_elim1 {L: Language} {nL: NormalLanguage L} {pL: PropositionalLanguage L} {sL: SeparationLanguage L} {s'L: SeparationEmpLanguage L} {MD: Model} {kMD: KripkeModel MD} (M: Kmodel) {R: Relation (Kworlds M)}  {po_R: PreOrder Krelation} {J: Join (Kworlds M)} {SA: SeparationAlgebra (Kworlds M)} {ISSSA: IncreasingSplitSmallerSeparationAlgebra (Kworlds M)} {SM: Semantics L MD} {kiSM: KripkeIntuitionisticSemantics L MD M SM} {fsSM: SeparatingSemantics L MD M SM} {feSM: EmpSemantics L MD M SM}:
+Lemma sound_emp_sepcon_elim1 {ISSSA: IncreasingSplitSmallerSeparationAlgebra (Kworlds M)}:
   forall x y: expr,
     forall m, KRIPKE: M, m |= x * y && emp --> x.
 Proof.
@@ -174,7 +210,7 @@ Proof.
   eapply sat_mono; eauto.
 Qed.
 
-Lemma sound_emp_dup {L: Language} {nL: NormalLanguage L} {pL: PropositionalLanguage L} {sL: SeparationLanguage L} {s'L: SeparationEmpLanguage L} {MD: Model} {kMD: KripkeModel MD} (M: Kmodel) {R: Relation (Kworlds M)}  {po_R: PreOrder Krelation} {J: Join (Kworlds M)} {SA: SeparationAlgebra (Kworlds M)} {IJSSA: IncreasingJoinSelfSeparationAlgebra (Kworlds M)} {SM: Semantics L MD} {kiSM: KripkeIntuitionisticSemantics L MD M SM} {fsSM: SeparatingSemantics L MD M SM} {feSM: EmpSemantics L MD M SM}:
+Lemma sound_emp_dup {IJSSA: IncreasingJoinSelfSeparationAlgebra (Kworlds M)}:
   forall x y: expr,
     forall m, KRIPKE: M, m |= x && emp --> x * x.
 Proof.
@@ -188,15 +224,4 @@ Proof.
   exists n, n; auto.
 Qed.
 
-Lemma sound_sepcon_elim1 {L: Language} {nL: NormalLanguage L} {pL: PropositionalLanguage L} {sL: SeparationLanguage L} {MD: Model} {kMD: KripkeModel MD} (M: Kmodel) {R: Relation (Kworlds M)}  {po_R: PreOrder Krelation} {J: Join (Kworlds M)} {SA: SeparationAlgebra (Kworlds M)} {incrSA: IncreasingSeparationAlgebra (Kworlds M)} {SM: Semantics L MD} {kiSM: KripkeIntuitionisticSemantics L MD M SM} {fsSM: SeparatingSemantics L MD M SM}:
-  forall x y: expr,
-    forall m, KRIPKE: M, m |= x * y --> x.
-Proof.
-  intros.
-  rewrite sat_impp; intros.
-  rewrite sat_sepcon in H0.
-  destruct H0 as [m1 [m2 [? [? ?]]]].
-  apply join_comm in H0.
-  apply all_increasing in H0.
-  eapply sat_mono; eauto.
-Qed.
+End Sound_Flat.
